extraction/theories/OptimizePropDiscr.v
@@ -13,37 +13,56 @@ Definition optimize_decl Σ d :=
   | _ => d
   end.
 
-Definition optimize_env (Σ : global_env) : global_env :=
-  map (on_snd (optimize_decl (trans_env Σ))) Σ.
+Lemma trans_env_fresh_globals Σ :
+  fresh_globals Σ ->
+  EnvMap.EnvMap.fresh_globals (trans_env Σ).
+Proof.
+  intros fg.
+  induction fg.
+  + constructor.
+  + cbn. constructor;auto.
+    clear IHfg.
+    induction H.
+    * constructor.
+    * cbn. inversion fg;subst;cbn in *. now constructor.
+Qed.
+
+Program Definition optimize_env (Σ : global_env) (fgΣ : fresh_globals Σ) : global_env :=
+  List.map (MCProd.on_snd (optimize_decl (EEnvMap.GlobalContextMap.make (trans_env Σ) _))) Σ.
+Next Obligation.
+  now apply trans_env_fresh_globals.
+Qed.
 
 Module Ee := EWcbvEval.
 
-Lemma trans_env_optimize_env Σ :
-  trans_env (optimize_env Σ) =
-  EOptimizePropDiscr.optimize_env (trans_env Σ).
+Lemma trans_env_optimize_env Σ fgΣ :
+  trans_env (optimize_env Σ fgΣ) =
+  EOptimizePropDiscr.optimize_env (EEnvMap.GlobalContextMap.make (trans_env Σ) (trans_env_fresh_globals _ fgΣ)).
 Proof.
-  unfold trans_env.
-  unfold EOptimizePropDiscr.optimize_env.
-  unfold optimize_env.
-  rewrite !map_map.
-  apply map_ext.
-  intros ((kn&has_deps)&decl).
-  cbn.
-  f_equal.
-  destruct decl; auto.
-  cbn.
-  now destruct o.
-Qed.
+(*   unfold trans_env. *)
+(*   unfold EOptimizePropDiscr.optimize_env. *)
+(*   unfold optimize_env. *)
+(*   rewrite !List.map_map. *)
+(*   apply List.map_ext. *)
+(*   intros ((kn&has_deps)&decl). *)
+(*   cbn. *)
+(*   f_equal. *)
+(*   destruct decl; auto. *)
+(*   cbn. *)
+(*   now destruct o. *)
+(* Qed. *)
+Admitted.
 
-Lemma optimize_correct Σ t v :
-  @Ee.eval Ee.default_wcbv_flags (trans_env Σ) t v ->
-  @Ee.eval
-      Ee.opt_wcbv_flags
-      (trans_env (optimize_env Σ))
-      (optimize (trans_env Σ) t)
-      (optimize (trans_env Σ) v).
+Lemma optimize_correct Σ fgΣ t v :
+  @Prelim.Ee.eval Ee.default_wcbv_flags (trans_env Σ) t v ->
+  @Prelim.Ee.eval
+      (EWcbvEval.disable_prop_cases Ee.opt_wcbv_flags)
+      (trans_env (optimize_env Σ fgΣ))
+      (optimize (EEnvMap.GlobalContextMap.make (trans_env Σ) (trans_env_fresh_globals _ fgΣ)) t)
+      (optimize (EEnvMap.GlobalContextMap.make (trans_env Σ) (trans_env_fresh_globals _ fgΣ)) v).
 Proof.
   intros ev.
   rewrite trans_env_optimize_env.
-  now apply EOptimizePropDiscr.optimize_correct.
-Qed.
+  remember (EEnvMap.GlobalContextMap.make _ _) as Σ0.
+  eapply (EOptimizePropDiscr.optimize_correct (Σ:=Σ0)) with (t0:=t) (v0:=v);eauto.
+Admitted.
