extraction/theories/CameLIGOExtract.v
@@ -1,3 +1,5 @@
+From Coq Require Import String.
+From Coq Require Import List.
 From ConCert.Execution Require Import Blockchain.
 From ConCert.Execution Require Import ContractCommon.
 From ConCert.Execution Require Import Serializable.
@@ -14,8 +16,10 @@ From ConCert.Extraction Require Import Utils.
 From ConCert.Extraction Require Import SpecializeChainBase.
 From ConCert.Utils Require Import Env.
 From MetaCoq.Template Require Import Kernames.
-From MetaCoq.Template Require Import All.
+From MetaCoq.Template Require monad_utils.
+From MetaCoq.Template Require Import TemplateMonad.
 
+Import monad_utils.MCMonadNotation ListNotations.
 
 Record CameLIGOMod {Base : ChainBase} (msg ctx setup storage operation : Type) :=
   { lmd_module_name : string ;
@@ -56,7 +60,7 @@ Definition cameligo_args :=
 
 Import PCUICAst PCUICTyping.
 Definition annot_extract_env_cameligo
-           (Σ : PCUICAst.global_env)
+           (Σ : PCUICEnvironment.global_env)
            (wfΣ : ∥wf Σ∥)
            (include : KernameSet.t)
            (ignore : list kername) : result (∑ Σ, env_annots box_type Σ) string.
@@ -71,14 +75,13 @@ Proof.
     * exact (Err e).
 Defined.
 
-
 Program Definition annot_extract_template_env_specalize
-           (e : TemplateEnvironment.global_env)
+           (e : Ast.Env.global_env)
            (seeds : KernameSet.t)
-           (ignore : list kername) : result (∑ e, env_annots box_type e) string :=
-  let e := SafeTemplateChecker.fix_global_env_universes e in
-  let e := TemplateToPCUIC.trans_global_decls e in
-  e <- specialize_ChainBase_env e ;;
+           (ignore : list kername) : result_string (∑ e, env_annots box_type e) :=
+  (* let e := SafeTemplateChecker.fix_global_env_universes e in *)
+  let e := TemplateToPCUIC.trans_global_env e in
+  e <- specialize_ChainBase_env (PCUICProgram.trans_env_env e) ;;
   wfe <-check_wf_env_func extract_within_coq e;;
   annot_extract_env_cameligo e wfe seeds ignore.
 
@@ -101,7 +104,9 @@ Definition CameLIGO_ignore_default {Base : ChainBase} :=
     ; <%% finalized_height %%>
   ].
 
-Definition TT_remap_default : list (kername * string) :=
+Open Scope string.
+
+Definition TT_remap_default : list (kername * String.string) :=
   [
     (* types *)
     remap <%% Z %%> "tez"
@@ -188,7 +193,7 @@ Definition TT_remap_default : list (kername * string) :=
   ; remap <%% @finalized_height %%> "finalized_height"
   ].
 
-Definition TT_rename_ctors_default : list (string * string) :=
+Definition TT_rename_ctors_default : list (String.string * String.string) :=
   [ ("nil", "[]")
   ; ("true", "true")
   ; ("false", "false")
@@ -197,7 +202,7 @@ Definition TT_rename_ctors_default : list (string * string) :=
   ; ("tt", "()")].
 
 Definition wrap_in_delimiters s :=
-  String.concat nl [""; s].
+  Strings.String.concat Common.nl [""; s].
 
 Definition is_empty {A} (xs : list A) :=
   match xs with
@@ -209,30 +214,35 @@ Section LigoExtract.
 
   Context `{ChainBase}
           `{CameLIGOPrintConfig}.
+
+  Open Scope list.
+
+  Notation "'bs_to_s' s" := (bytestring.String.to_string s) (at level 200).
+  Local Coercion bytestring.String.to_string : bytestring.String.t >-> String.string.
   
 Definition printCameLIGODefs {msg ctx params storage operation : Type}
-           (Σ : TemplateEnvironment.global_env)
-           (TT_defs : list (kername *  string))
-           (TT_ctors : env string)
+           (Σ : Ast.Env.global_env)
+           (TT_defs : list (kername *  String.string))
+           (TT_ctors : env String.string)
            (extra_ignore : list kername)
-           (build_call_ctx : string)
+           (build_call_ctx : String.string)
            (init : kername)
            (receive : kername)
            (m : CameLIGOMod msg ctx params storage operation)
-  : string + string :=
+  : String.string + String.string :=
   let init_prelude := m.(lmd_init_prelude) in
   let entry_point := m.(lmd_entry_point) in
   let seeds := KernameSet.union (KernameSet.singleton init) (KernameSet.singleton receive) in
   let TT_defs := TT_defs ++ TT_remap_default in
   let ignore := (map fst TT_defs ++ CameLIGO_ignore_default ++ extra_ignore)%list in
   let TT :=
-      (TT_ctors ++ map (fun '(kn,d) => (string_of_kername kn, d)) TT_defs)%list in
+      (TT_ctors ++ map (fun '(kn,d) => (bs_to_s (string_of_kername kn), d)) TT_defs)%list in
   match annot_extract_template_env_specalize Σ seeds ignore with
   | Ok (eΣ; annots) =>
     (* dependencies should be printed before the dependent definitions *)
     let ldef_list := List.rev (print_global_env TT eΣ annots) in
     (* filtering empty strings corresponding to the ignored definitions *)
-    let not_empty_str := (negb ∘ (String.eqb "") ∘ snd) in
+    let not_empty_str := (negb ∘ (Strings.String.eqb "") ∘ snd) in
 
     let ldef_ty_list := ldef_list
                           |> filter (fun d => match d with TyDecl _ => true | _ => false end)
@@ -249,34 +259,36 @@ Definition printCameLIGODefs {msg ctx params storage operation : Type}
       | Some init_code =>
         (* filtering out the definition of [init] and projecting the code *)
         (* and place init prelude after type decls and before constant decls *)
-        let defs : list string :=
+        let defs : list String.string :=
           ldef_const_list |> filter (negb ∘ (eq_kername init) ∘ fst)
                           |> map snd
                           |> List.app (map snd ldef_ty_list) (* append the above after ty decls*)
                           in
-        let res : string :=
-            String.concat (nl ++ nl) (defs ++ (cons init_code nil)) in
-        (wrap_in_delimiters (String.concat (nl ++ nl) [m.(lmd_prelude); res; entry_point])) |> inl
+        let res : String.string :=
+            Strings.String.concat (Common.nl ++ Common.nl) (defs ++ (cons init_code nil)) in
+        (wrap_in_delimiters (Strings.String.concat (Common.nl ++ Common.nl) [m.(lmd_prelude); res; entry_point])) |> inl
       | None => inr "Error: Empty body for init"
       end
     | Some _ => inr "Error: init must be a constant"
     | None => inr "Error: No init found"
     end
-  | Err e => inr e
+  | Err e => inr (bs_to_s e)
   end.
 
 
-Definition unwrap_string_sum (s : string + string) : string :=
+Definition unwrap_string_sum (s : String.string + String.string) : String.string :=
   match s with
   | inl v => v
   | inr v => v
   end.
 
+Open Scope bs_scope.
+
 Definition quote_and_preprocess {Base : ChainBase}
            {msg ctx params storage operation : Type}
            (inline : list kername)
            (m : CameLIGOMod msg ctx params storage operation)
-  : TemplateMonad (TemplateEnvironment.global_env * kername * kername) :=
+  : TemplateMonad (Ast.Env.global_env * kername * kername) :=
    (* we compute with projections before quoting to avoid unnecessary dependencies to be quoted *)
    init <- tmEval cbn m.(lmd_init);;
    receive <-tmEval cbn m.(lmd_receive);;
@@ -301,59 +313,60 @@ Definition quote_and_preprocess {Base : ChainBase}
     which is much faster than running the computations inside [TemplateMonad]. *)
 Definition CameLIGO_prepare_extraction {msg ctx params storage operation : Type}
            (inline : list kername)
-           (TT_defs : list (kername *  string))
-           (TT_ctors : env string)
+           (TT_defs : list (kername * String.string))
+           (TT_ctors : env String.string)
            (extra_ignore : list kername)
-           (build_call_ctx : string)
+           (build_call_ctx : String.string)
            (m : CameLIGOMod msg ctx params storage operation) :=
   '(Σ, init_nm, receive_nm) <- quote_and_preprocess inline m;;
-  let TT_defs := TT_defs ++ TT_remap_default in
+  let TT_defs := (TT_defs ++ TT_remap_default)%list in
   let TT :=
-      (TT_ctors ++ map (fun '(kn,d) => (string_of_kername kn, d)) TT_defs)%list in
+      (TT_ctors ++ map (fun '(kn,d) => (bs_to_s (string_of_kername kn), d)) TT_defs)%list in
   let res := unwrap_string_sum (printCameLIGODefs Σ TT_defs TT_ctors extra_ignore
                                                   build_call_ctx
                                                   init_nm receive_nm
                                                   m) in
-  tmDefinition (m.(lmd_module_name) ^ "_prepared") res.
+  tmDefinition (bytestring.String.of_string m.(lmd_module_name) ^ "_prepared") res.
 
 (** Bundles together quoting, inlining, erasure and pretty-printing.
     Convenient to use, but might be slow, becase performance of [tmEval lazy] is not great. *)
 Definition CameLIGO_extract {msg ctx params storage operation : Type}
            (inline : list kername)
-           (TT_defs : list (kername *  string))
-           (TT_ctors : env string)
+           (TT_defs : list (kername *  String.string))
+           (TT_ctors : env String.string)
            (extra_ignore : list kername)
-           (build_call_ctx : string)
-           (m : CameLIGOMod msg ctx params storage operation) :=
+           (build_call_ctx : String.string)
+           (m : CameLIGOMod msg ctx params storage operation) : TemplateMonad String.string:=
   '(Σ, init_nm, receive_nm) <- quote_and_preprocess inline m;;
-  let TT_defs := TT_defs ++ TT_remap_default in
+  let TT_defs := (TT_defs ++ TT_remap_default)%list in
   let TT :=
-      (TT_ctors ++ map (fun '(kn,d) => (string_of_kername kn, d)) TT_defs)%list in
+      (TT_ctors ++ map (fun '(kn,d) => (bs_to_s (string_of_kername kn), d)) TT_defs)%list in
   p <- tmEval lazy
              (printCameLIGODefs Σ TT_defs TT_ctors extra_ignore
                                 build_call_ctx
                                 init_nm receive_nm
                                 m) ;;
-  match p with
+  match (p : String.string + String.string) with
   | inl s =>
     tmEval lazy
-           (wrap_in_delimiters (String.concat (nl ++ nl) [m.(lmd_prelude); s; m.(lmd_entry_point)]))
-  | inr s => tmFail s
+           (wrap_in_delimiters (Strings.String.concat (Common.nl ++ Common.nl)
+                                              [m.(lmd_prelude); s; m.(lmd_entry_point)]))
+  | inr s => tmFail (bytestring.String.of_string s)
   end.
 
 (** A simplified erasure/prinitng intended moslty for testing purposes *)
-Definition simple_def_print `{ChainBase} TT_defs TT_ctors seeds prelude harness Σ
-  : string + string :=
-  let TT_defs := TT_defs ++ TT_remap_default in
+Definition simple_def_print `{ChainBase} TT_defs TT_ctors seeds (prelude harness : String.string) Σ
+  : String.string + String.string :=
+  let TT_defs := (TT_defs ++ TT_remap_default)%list in
   let ignore := (map fst TT_defs ++ CameLIGO_ignore_default)%list in
-  let TT := (TT_ctors ++ map (fun '(kn,d) => (string_of_kername kn, d)) TT_defs)%list in
+  let TT := (TT_ctors ++ map (fun '(kn,d) => (bs_to_s (string_of_kername kn), d)) TT_defs)%list in
   match annot_extract_template_env_specalize Σ seeds ignore with
   | Ok annot_env =>
   let '(eΣ; annots) := annot_env in
       (* dependencies should be printed before the dependent definitions *)
   let ldef_list := List.rev (print_global_env TT eΣ annots) in
     (* filtering empty strings corresponding to the ignored definitions *)
-    let not_empty_str := (negb ∘ (String.eqb "") ∘ snd) in
+    let not_empty_str := (negb ∘ (Strings.String.eqb "") ∘ snd) in
 
     let ldef_ty_list := ldef_list
                           |> filter (fun d => match d with TyDecl _ => true | _ => false end)
@@ -363,11 +376,11 @@ Definition simple_def_print `{ChainBase} TT_defs TT_ctors seeds prelude harness 
                             |> filter (fun d => match d with ConstDecl _ => true | _ => false end)
                             |> map (fun d => match d with ConstDecl d' => d' | TyDecl d' => d' end)
                             |> filter not_empty_str in
-    let defs : list string :=
+    let defs : list String.string :=
         ldef_const_list  |> map snd
                          |> List.app (map snd ldef_ty_list) in
-    String.concat (nl ^ nl) (prelude :: defs ++ [harness]) |> inl
-  | Err e => inr e
+    Strings.String.concat (Common.nl ++ Common.nl) ((prelude :: defs ++ [harness]))%list |> inl
+  | Err e => inr (bs_to_s e)
   end.
 
 (** Quoting and inlining for a single definition.
@@ -375,7 +388,7 @@ Definition simple_def_print `{ChainBase} TT_defs TT_ctors seeds prelude harness 
 Definition quote_and_preprocess_one_def {A}
            (inline : list kername)
            (def : A)
-  : TemplateMonad (TemplateEnvironment.global_env * kername) :=
+  : TemplateMonad (Ast.Env.global_env * kername) :=
   '(Σ,_) <- tmQuoteRecTransp def false ;;
   def_nm <- extract_def_name def;;
   Σ <-(if is_empty inline then ret Σ
@@ -394,11 +407,11 @@ Definition quote_and_preprocess_one_def {A}
     of [storage], [main], etc.*)
 Definition CameLIGO_extract_single `{ChainBase} {A}
            (inline : list kername)
-           (TT_defs : list (kername *  string))
-           (TT_ctors : env string)
-           (prelude : string)
-           (harness: string)
-           (def : A) : TemplateMonad string :=
+           (TT_defs : list (kername *  String.string))
+           (TT_ctors : env String.string)
+           (prelude : String.string)
+           (harness: String.string)
+           (def : A) : TemplateMonad String.string :=
   '(Σ,def_nm) <- quote_and_preprocess_one_def inline def ;;
   let seeds := KernameSetProp.of_list [def_nm] in
   tmEval lazy (unwrap_string_sum (simple_def_print TT_defs TT_ctors (KernameSet.singleton def_nm) prelude harness Σ)).
@@ -406,11 +419,11 @@ Definition CameLIGO_extract_single `{ChainBase} {A}
 (** Similar to [CameLIGO_prepare_extraction], but for a single definition  *)
 Definition CameLIGO_prepare_extraction_single `{ChainBase} {A}
            (inline : list kername)
-           (TT_defs : list (kername *  string))
-           (TT_ctors : env string)
-           (prelude : string)
-           (harness: string)
-           (def : A) : TemplateMonad string :=
+           (TT_defs : list (kername *  String.string))
+           (TT_ctors : env String.string)
+           (prelude : String.string)
+           (harness: String.string)
+           (def : A) : TemplateMonad String.string :=
     '(Σ,def_nm) <- quote_and_preprocess_one_def inline def ;;
     let seeds := KernameSetProp.of_list [def_nm] in
     tmDefinition (def_nm.2 ^ "_prepared") (unwrap_string_sum (simple_def_print TT_defs TT_ctors (KernameSet.singleton def_nm) prelude harness Σ)).
