extraction/theories/Common.v
@@ -1,3 +1,4 @@
+From Coq Require Import String.
 From ConCert.Extraction Require Import ResultMonad.
 From MetaCoq.Template Require Import Ast.
 From MetaCoq.Template Require Import LiftSubst.
@@ -8,6 +9,7 @@ From MetaCoq.Template Require Import Typing.
 From MetaCoq.Template Require Import utils.
 From MetaCoq.Erasure Require EAst.
 From MetaCoq.SafeChecker Require Import PCUICSafeChecker.
+From MetaCoq.SafeChecker Require Import PCUICWfEnvImpl.
 
 Import PCUICErrors.
 Import MCMonadNotation.
@@ -51,7 +53,7 @@ Definition result_of_typing_result
            (Σ : PCUICAst.PCUICEnvironment.global_env_ext)
            (tr : typing_result A) : result A string :=
   match tr with
-  | Checked a => ret a
+  | Checked a => Ok a
   | TypeError err => Err (string_of_type_error Σ err)
   end.
 
@@ -64,15 +66,15 @@ Definition string_of_env_error Σ e :=
   | AlreadyDeclared s => "Alreadydeclared " ++ s
   end.
 
-Definition result_of_EnvCheck {A} (ec : EnvCheck A) : result A string :=
-  match ec with
-  | CorrectDecl a => ret a
-  | EnvError Σ err => Err (string_of_env_error Σ err)
-  end.
+(* Definition result_of_EnvCheck {AS A} (ec : EnvCheck AS A) : result A string := *)
+(*   match ec with *)
+(*   | CorrectDecl a => ret a *)
+(*   | EnvError Σ err => Err (string_of_env_error Σ err) *)
+(*   end. *)
 
 Definition result_of_option {A} (o : option A) (err : string) : result A string :=
   match o with
-  | Some a => ret a
+  | Some a => Ok a
   | None => Err err
   end.
 
@@ -111,14 +113,14 @@ Definition extract_def_name_exists {A : Type} (a : A) : TemplateMonad kername :=
 Notation "'unfolded' d" :=
   ltac:(let y := eval unfold d in d in exact y) (at level 100, only parsing).
 
-Definition remap (kn : kername) (new_name : string) : kername * string :=
+Definition remap (kn : kername) (new_name : String.string) : kername * String.string :=
   (kn, new_name).
 
-Definition EnvCheck_to_template {A } (ec : EnvCheck A) : TemplateMonad A :=
-  match ec with
-  | CorrectDecl a => ret a
-  | EnvError Σ e => tmFail (string_of_env_error Σ e)
-  end.
+(* Definition EnvCheck_to_template { AS A} (ec : EnvCheck AS A) : TemplateMonad A := *)
+(*   match ec with *)
+(*   | CorrectDecl a => ret a *)
+(*   | EnvError Σ e => tmFail (string_of_env_error Σ e) *)
+(*   end. *)
 
 Definition quote_recursively_body {A : Type} (def : A) : TemplateMonad program :=
   p <- tmQuoteRecTransp def false ;;
@@ -279,3 +281,25 @@ Definition Z_syn_to_Z (t : EAst.term) : option Z :=
     else None
   | _ => None
   end.
+
+(* TODO: port the pretty-printers to use bytestring and use metacoq's MCString utils *)
+
+Definition parens (top : bool) (s : String.string) : String.string :=
+  if top then s else  "(" ++ s ++ ")".
+
+Definition nl : String.string := String (Ascii.ascii_of_nat 10) EmptyString.
+
+Definition string_of_list_aux {A} (f : A -> String.string) (sep : String.string) (l : list A) : String.string :=
+  let fix aux l :=
+      match l return String.string with
+      | nil => ""%string
+      | cons a nil => f a
+      | cons a l => (f a ++ sep ++ aux l)%string
+      end
+  in aux l.
+
+Definition string_of_list {A} (f : A -> String.string) (l : list A) : String.string :=
+  ("[" ++ string_of_list_aux f "," l ++ "]")%string.
+
+Definition print_list {A} (f : A -> String.string) (sep : String.string) (l : list A) : String.string :=
+  string_of_list_aux f sep l.
