extraction/theories/ConcordiumExtract.v
@@ -1,4 +1,4 @@
-From MetaCoq Require Import utils.
+(* From MetaCoq Require Import utils. *)
 From MetaCoq.Template Require Import All.
 From MetaCoq.Template Require Import Kernames.
 From ConCert.Utils Require Import StringExtra.
@@ -12,6 +12,18 @@ From ConCert.Extraction Require Import PrettyPrinterMonad.
 From ConCert.Extraction Require Import Printing.
 From ConCert.Extraction Require Import ResultMonad.
 From ConCert.Extraction Require Import Utils.
+From Coq Require Import List.
+From Coq Require Import String.
+From Coq Require Import ZArith.
+
+Import MCMonadNotation.
+
+Local Open Scope string_scope.
+Local Notation bs_to_s := bytestring.String.to_string.
+Local Notation s_to_bs := bytestring.String.of_string.
+
+Local Coercion bytestring.String.of_string : string >-> bytestring.string.
+
 
 Module ConcordiumRemap.
 
@@ -222,7 +234,7 @@ Definition build_remaps
 End ConcordiumRemap.
 
 Module ConcordiumPreamble.
-  Instance concordium_extract_preamble : Preamble :=
+  Local Instance concordium_extract_preamble : Preamble :=
 {| top_preamble := [
 "#![allow(dead_code)]";
 "#![allow(unused_imports)]";
@@ -372,8 +384,11 @@ Definition get_fn_arg_type (Σ : Ex.global_env) (fn_name : kername) (n : nat)
   match Ex.lookup_env Σ fn_name with
   | Some (Ex.ConstantDecl cb) =>
     match decompose_TArr cb.(Ex.cst_type).2 with
-    | (tys, _) => result_of_option (nth_error tys n)
-                                  ("No argument at position " ++ string_of_nat n)
+    | (tys, _) =>
+        match nth_error tys n with
+        | Some v => Ok v
+        | None => Err("No argument at position " ++ string_of_nat n)
+        end
     end
   | _ => Err "Init declaration must be a constant in the global environment"
   end.
@@ -382,7 +397,7 @@ Definition specialize_extract_template_env
            (params : extract_template_env_params)
            (Σ : global_env)
            (seeds : KernameSet.t)
-           (ignore : kername -> bool) : result ExAst.global_env string :=
+           (ignore : kername -> bool) : result ExAst.global_env _ :=
   extract_template_env_general SpecializeChainBase.specialize_ChainBase_env
                        params
                        Σ
@@ -393,11 +408,15 @@ Section ConcordiumPrinting.
 
   Context `{RustPrintConfig}.
 
+  Definition result_string_err A := result A bytestring.string.
+
+  Existing Instance ConcordiumPreamble.concordium_extract_preamble.
+
   Definition extract_lines
              (seeds : KernameSet.t)
              (Σ : global_env)
              (remaps : remaps)
-             (params : extract_template_env_params) : result (list string) string :=
+             (params : extract_template_env_params) : result_string_err (list string) :=
     let should_ignore kn :=
         if remap_inductive remaps (mkInd kn 0) then true else
         if remap_constant remaps kn then true else
@@ -405,7 +424,7 @@ Section ConcordiumPrinting.
     Σ <- specialize_extract_template_env params Σ seeds should_ignore;;
     let attrs _ := "#[derive(Clone, ConCertSerial, ConCertDeserial, PartialEq)]" in
     let p := print_program Σ remaps attrs in
-    '(_, s) <- timed "Printing" (fun _ => finish_print_lines p);;
+    '(_, s) <- timed "Printing" (fun _ => map_error s_to_bs (finish_print_lines p));;
     ret s.
 
   Open Scope string.
@@ -535,14 +554,16 @@ Section ConcordiumPrinting.
      "    }";
 "}" $>.
 
-  Definition print_lines (lines : list string) : TemplateMonad unit :=
+  Definition print_lines (lines : list bytestring.string) : TemplateMonad unit :=
     monad_iter tmMsg lines.
+
+Open Scope bool.
 
 Definition concordium_extraction
            {init_type receive_type : Type}
            (m : ConcordiumMod init_type receive_type)
            (remaps : remaps)
-           (should_inline : kername -> bool) : TemplateMonad _ :=
+           (should_inline : kername -> bool) : TemplateMonad unit :=
   init_tm <- tmEval cbn m.(concmd_init);;
   recv_tm <- tmEval cbn m.(concmd_receive);;
   '(Σ,_) <- tmQuoteRecTransp (init_tm, recv_tm) false ;;
@@ -562,7 +583,7 @@ Definition concordium_extraction
   | Ok lines =>
     let init_wrapper := init_wrapper m.(concmd_contract_name) init_nm in
     let receive_wrapper := receive_wrapper m.(concmd_contract_name) receive_nm in
-    print_lines (lines ++ [""; init_wrapper; ""; convert_actions; ""; receive_wrapper])
+    print_lines (map s_to_bs (lines ++ [""; init_wrapper; ""; convert_actions; ""; receive_wrapper]))
   | Err e => tmFail e
   end.
 
